src/Completeness.v
@@ -9,13 +9,14 @@ Require Import Relation_Operators.
 Require Import Coq.Setoids.Setoid.
 Require Import Typing.
 Require Import Infer.
-Require Import MoreGeneral.
 Require Import NewTypeVariable.
+Require Import MoreGeneral.
 
 Require Import LibTactics.
 
-Lemma id_increases_in_w : forall (e : term) (i i' : id) (G : ctx) (tau : ty) (s : substitution),
-                            getResult (runInfer_id e G i) = Some (i', tau, s) -> i <= i'.
+Lemma id_increases_in_w : forall (e : term) (i i' : id) (G : ctx) (tau : ty)
+    (s : substitution),
+    getResult (runInfer_id e G i) = Some (i', tau, s) -> i <= i'.
 Admitted.
 
 Lemma new_tv_W: forall (e : term) (G : ctx) (i i': id) (t : ty) (s : substitution),
@@ -25,6 +26,20 @@ Admitted.
 
 Lemma completeness : forall (e : term) (G : ctx) (tau' : ty) (phi : substitution) (i : id),
     has_type (apply_subst_ctx phi G) e tau' -> new_tv_ctx G i ->
-    exists s tau i' s', getResult (runInfer_id e G i) = Some (i', tau, s) /\ tau' = apply_subst s' tau /\
-                   (forall x : id, x < i -> apply_subst phi (var x) = apply_subst (s ++ s') (var x)).
+    exists s tau i' s', getResult (runInfer_id e G i) = Some (i', tau, s) /\
+    tau' = apply_subst s' tau /\
+    (forall x : id, x < i -> apply_subst phi (var x) = apply_subst (s ++ s') (var x)).
+Proof.
+  intros.
+  induction e.
+  admit.
+  admit.
+  admit.
+  admit.
+  - inversion H.
+    simpl.
+    (** rever a parte do algoritmo que infere constantes *)
+    exists (nil : substitution) (con 0) i (nil : substitution).
+    simpl. split; try reflexivity.
+
 Admitted.
